Use stdlib fmap

coq/perm/Solver.v
@@ -17,7 +17,7 @@ Local Existing Instance config.default_checker_flags.
 
 From Graph Require Import Bij SigPerm.
 
-From stdpp Require Import base.
+From stdpp Require Import base countable fin_maps gmap gmultiset.
 
 
 
@@ -63,13 +63,13 @@ Definition A := nat.
 (* TODO: Trivial example: Without variable for constants *)
 (* TODO: First implement this when constant is nat *)
 Inductive atom :=
-| avar (x : var) : atom
-| alit (c : A) : atom.
+| A_lit (c : A) : atom
+| A_var (x : var) : atom.
 
 Inductive atyp :=
+| AT_nil : atyp 
 | AT_atom (a : atom) : atyp
 | AT_var (x : var)  : atyp
-| AT_nil : atyp 
 .
 
 Definition lform := list atyp.
@@ -120,12 +120,15 @@ Definition size_lform (f : lform) :=
 
 Inductive peqn :=
 | PE_perm (l1 l2 : lform) : peqn
-| PE_aeq (a1 a2 : atom) : peqn.
+| PE_aeq (a1 a2 : atom) : peqn
+| PE_false
+.
 
 Definition size_peqn (p : peqn) :=
   match p with
   | PE_perm l1 l2 => size_lform l1 + size_lform l2
   | PE_aeq a1 a2 => 2
+  | PE_false => 1
   end.
 
 (* TODO: Not sure this helps *)
@@ -157,6 +160,7 @@ Definition peqn_comm (p : peqn) :=
   match p with
   | PE_perm l1 l2 => PE_perm l2 l1
   | PE_aeq a1 a2 => PE_aeq a2 a1
+  | PE_false => PE_false
   end.
 
 (* TODO: Whether I want to also do comm equiv or not, but maybe this strict version is fine *)
@@ -166,30 +170,36 @@ Definition peqn_equiv (p1 p2 : peqn) : Prop :=
       l11 ≡[P] l21 /\ l12 ≡[P] l22
   | PE_aeq a11 a12, PE_aeq a21 a22 =>
       a11 = a21 /\ a12 = a22
+  | PE_false, PE_false => True
   | _, _ => False
   end.
 
 Import ConvertTactics.
 
-Lemma perm_peqn_dec (l1 l2 : lform) : {l1 ≡[P] l2}+{~(l1 ≡[P] l2)}.
-Proof.
-  revert l2.
-  induction l1; destruct l2.
-  - left. reflexivity.
-  - right. intros Hcontra.
-    apply Permutation_rel_length in Hcontra. discriminate.
-  - right. intros Hcontra.
-    apply Permutation_rel_length in Hcontra. discriminate.
-  - pose proof EqDecision_atyp. destruct (decide_rel eq a a0).
-    + specialize (IHl1 l2). destruct IHl1.
-      * left. convert_mfperm.
-        subst.
-        apply Permutation_rel_cons. auto.
-      * right. intros Hcontra. subst.
-        apply Permutation_rel_cons_inv in Hcontra. auto.
-    + admit.
-Admitted.
+(* Lemma perm_peqn_dec (l1 l2 : lform) : {l1 ≡[P] l2}+{~(l1 ≡[P] l2)}. *)
+(* Proof. *)
+(*   revert l2. *)
+(*   induction l1; destruct l2. *)
+(*   - left. reflexivity. *)
+(*   - right. intros Hcontra. *)
+(*     apply Permutation_rel_length in Hcontra. discriminate. *)
+(*   - right. intros Hcontra. *)
+(*     apply Permutation_rel_length in Hcontra. discriminate. *)
+(*   - pose proof EqDecision_atyp. destruct (decide_rel eq a a0). *)
+(*     + specialize (IHl1 l2). destruct IHl1. *)
+(*       * left. convert_mfperm. *)
+(*         subst. *)
+(*         apply Permutation_rel_cons. auto. *)
+(*       * right. intros Hcontra. subst. *)
+(*         apply Permutation_rel_cons_inv in Hcontra. auto. *)
+(*     + admit. *)
+(* Admitted. *)
 
+(* TODO: This is a bit restricted, but maybe this is the right notion *)
+Lemma peqn_dec (p1 p2 : peqn) : {p1 = p2} + {~(p1 = p2)}.
+Proof.
+  repeat decide equality.
+Defined.
 
 (** Substitution *)
 (* TODO: substitution replacing var with var or Prop *)
@@ -200,77 +210,423 @@ Definition subst_var_atyp (v v' : var) (t : atyp) : atyp :=
   | AT_atom c => AT_atom c
   end.
 
-Definition subst_var_atom (v v' : var) (a : atom) : atom :=
+Definition subst_avar_atom (v v' : var) (a : atom) : atom :=
   match a with
-  | avar x => if eq_dec x v then avar v' else avar x
-  | alit i => alit i
+  | A_var x => if eq_dec x v then A_var v' else A_var x
+  | A_lit i => A_lit i
   end.
 
-Definition subst_atom_atyp (f : atom -> atom) (t : atyp) : atyp :=
+Definition subst_avar_atyp (v v' : var) (t : atyp) : atyp :=
   match t with
   | AT_var x => AT_var x
   | AT_nil => AT_nil
-  | AT_atom c => AT_atom (f c)
+  | AT_atom c => AT_atom (subst_avar_atom v v' c)
   end.
 
-Definition subst_atyp_lform (f : atyp -> atyp) : lform -> lform :=
-  List.map f.
+Definition subst_var_lform (v v' : var) : lform -> lform :=
+  List.map (subst_var_atyp v v').
 
-(* Definition subst_atom_lform (f : atom -> atom) : lform -> lform := *)
-(*   List.map (subst_atom_atyp f). *)
+Definition subst_avar_lform (v v' : var) : lform -> lform :=
+  List.map (subst_avar_atyp v v').
 
-Definition subst_atyp_peqn (f : atyp -> atyp) (eqn : peqn) : peqn :=
-  match eqn with
+Definition subst_var_peqn (v v' : var) (p : peqn) : peqn :=
+  match p with
   | PE_perm l1 l2 =>
-      PE_perm (subst_atyp_lform f l1) (subst_atyp_lform f l2)
+      PE_perm (subst_var_lform v v' l1) (subst_var_lform v v' l2)
   | PE_aeq a1 a2 => PE_aeq a1 a2
+  | PE_false => PE_false
   end.
 
-Definition subst_atom_peqn (f : atom -> atom) (eqn : peqn) : peqn :=
-  match eqn with
+Definition subst_avar_peqn (v v' : var) (p : peqn) : peqn :=
+  match p with
   | PE_perm l1 l2 =>
-      PE_perm (subst_atyp_lform l1) l2
-  | PE_aeq a1 a2 => PE_aeq a1 a2
+      PE_perm (subst_avar_lform v v' l1) (subst_avar_lform v v' l2)
+  | PE_aeq a1 a2 => PE_aeq (subst_avar_atom v v' a1) (subst_avar_atom v v' a2)
+  | PE_false => PE_false
   end.
-      
 
+Definition subst_peqn (var_bindings : list (var * var)) (avar_bindings : list (var * var)) (p : peqn) : peqn :=
+  let p' := List.fold_left (fun acc '(v, v') => subst_var_peqn v v' acc) var_bindings p in
+  List.fold_left (fun acc '(v, v') => subst_avar_peqn v v' acc) avar_bindings p'.
 
-Definition plform_valid (p : plform) :=
-  Pleft p ≡[P] Pright p.
-
-Definition subst_var_plform (f : var -> var) (p : plform) : plform :=
-  mkPlform (subst_var_lform f (Pleft p)) (subst_var_lform f (Pright p)).
+Definition peqn_valid (p : peqn) :=
+  match p with
+  | PE_perm l1 l2 =>
+      l1 ≡[P] l2
+  | PE_aeq a1 a2 => a1 = a2
+  | PE_false => False
+  end.
 
 Definition valid s :=
-  forall f, (forall h, In h (hyps s) -> plform_valid (subst_var_plform f h)) -> plform_valid (subst_var_plform f (concl s)).
+  forall vb avb, (forall h, In h (hyps s) -> peqn_valid (subst_peqn vb avb h)) -> peqn_valid (subst_peqn vb avb (concl s)).
 
+Definition is_leaf s :=
+  let cl := concl s in
+  let dec_leaf h :=
+    if peqn_dec PE_false h then true else
+      if peqn_dec h cl then true else false
+  in
+  List.fold_left (fun b h => orb b (dec_leaf h)) (hyps s) false.
 
-Lemma perm_plform_dec (p1 p2 : plform) : {plform_equiv p1 p2}+{not (plform_equiv p1 p2)}.
+Lemma subst_PE_false_reflexive :
+  forall vb avb, subst_peqn vb avb PE_false = PE_false.
 Proof.
+  intros vb.
+  unfold subst_peqn.
+  induction vb; intros; simpl.
+  - induction avb; simpl; auto.
+    destruct a.
+    rewrite IHavb. simpl. auto.
+  - destruct a. apply IHvb.
+Qed.
+
+Lemma is_leaf_sound_in h hs:
+  valid {| hyps := h :: hs; concl := h |}.
+Proof.
+  red; simpl; intros.
+  assert (h = h \/ In h hs) by intuition.
+  apply H in H0; auto.
+Qed.
+  (* H : valid {| hyps := h; concl := cl |} *)
+  (* ============================ *)
+(* valid {| hyps := PE_perm l1 l2 :: h; concl := cl |} *)
+
+Lemma valid_weakening : forall h hs cl,
+  valid {| hyps := hs; concl := cl|} ->
+  valid {| hyps := h :: hs; concl := cl|}.
+Proof.
+  unfold valid. intros.
+  apply H.
+  intros; simpl in *.
+  assert (Hin: h = h0 \/ In h0 hs) by intuition.
+  apply H0 in Hin; intuition.
+Qed.
+
+Lemma valid_ex_falso : forall hs cl,
+    valid {| hyps := PE_false :: hs; concl := cl |}.
+Proof.
+  red; intros; simpl in *.
+  assert (H' :  PE_false = PE_false \/ In PE_false hs) by intuition.
+  apply H in H'. red in H'. rewrite subst_PE_false_reflexive in H'. destruct H'.
+Qed.
   
+Lemma is_leaf_sound s :
+  is_leaf s = true -> valid s.
+Proof.
+  unfold is_leaf.
+  destruct s as (h, cl); simpl. revert cl.
+  induction h; simpl; intros.
+  discriminate.
+  destruct a.
+  - destruct (peqn_dec (PE_perm l1 l2) cl).
+    + subst. apply is_leaf_sound_in.
+    + apply IHh in H. apply valid_weakening; intuition.
+  - destruct (peqn_dec (PE_aeq a1 a2) cl).
+    + subst. apply is_leaf_sound_in.
+    + apply IHh in H. apply valid_weakening; intuition.
+  - apply valid_ex_falso.
+Qed.
 
+Definition subgoal := list (list seq).
 
+(* TODO: Check this *)
+Definition valid_subgoal (sg:subgoal) :=
+  exists2 sl, In sl sg & forall s, In s sl -> valid s.
 
+Fixpoint pick {A} (h : list A) :=
+  match h with
+  | nil => nil
+  | a :: l =>
+      (a, l)::List.map (fun p => (fst p, a :: snd p)) (pick l)
+  end.
 
-(* Aggregate List *)
-Section AList.
-  Variable (A : Type).
-  (* We need:
-     1. A map from constants to number of occurrence
-     2. A map from variable constants to number of occurrence
-     3. A map from List variables to number of occurrence
-   *)
+Inductive result := Valid | CounterModel | Abort.
+
+(* HXC: I need a semantic for reasoning
+   In the example we are given a type class that takes in a type and have different semantics for them
+ *)
+(* Algorithm *)
+(* Step 1:
+Reduce to normal form i.e. if one side has some coefficient, the other side should not have coefficient
+
+1. Transform into a bag form
+2. Proof the identity rule
+ *)
+
+(* First define countable instances for var, atom, and atyp *)
+(* Increment by 1 so maintain uniqueness *)
+Definition encode_var (x : var) : positive :=
+  Pos.of_succ_nat x.
+
+Definition decode_var (p : positive) : option var :=
+  Some (Pos.to_nat p - 1).
+
+#[global]
+  Program Instance Countable_var : Countable var :=
+  {| encode := encode_var;
+    decode := decode_var
+  |}.
+Next Obligation.
+  intros.
+  unfold decode_var, encode_var.
+  rewrite SuccNat2Pos.id_succ. simpl.
+  rewrite Nat.sub_0_r. reflexivity.
+Defined.
+
+Section CountableInstances.
+  Context `{Countable A}.
+  Definition encode_atom (a : atom) : positive :=
+    match a with
+    | A_var v => (encode v)~0
+    | A_lit a => (encode a)~1
+    end.
+
+  Definition decode_atom (p : positive) : option atom :=
+    match p with
+    | xH => None
+    | xO p => A_var <$> (decode p)
+    | xI p => A_lit <$> (decode p)
+    end.
+
+    Global Program Instance Countable_atom : Countable atom :=
+    {| encode := encode_atom;
+      decode := decode_atom
+    |}.
+  Next Obligation.
+    intros. unfold decode_atom, encode_atom. destruct x.
+    - rewrite decode_encode. auto.
+    - rewrite decode_encode. auto.
+  Defined.
+
+  Definition encode_atyp (a : atyp) : positive :=
+    match a with
+    | AT_atom a => (encode a)~0
+    | AT_var v => (encode v)~1
+    | AT_nil => 1
+    end.
+
+  Definition decode_atyp (p : positive) : option atyp :=
+    match p with
+    | xH => Some AT_nil
+    | xO p => AT_atom <$> (decode p)
+    | xI p => AT_var <$> (decode p)
+    end.
+
+    Global Program Instance Countable_atyp : Countable atyp :=
+    {| encode := encode_atyp;
+      decode := decode_atyp
+    |}.
+    Next Obligation.
+      intros. unfold decode_atyp, encode_atyp.
+      destruct x; try rewrite decode_encode; simpl; auto.
+    Defined.
+
+    Global Program Instance Insert_atyp_gmultiset : Insert atyp nat (gmultiset A).
+    Next Obligation.
+    Admitted.
+    
+    Global Program Instance SingletonMS_atyp_gmultiset : SingletonMS atyp (gmultiset A) := fun a => <[ a := 1 ]> ∅.
+    
+End CountableInstances.
+
+From Coq Require Import
+  FSets.FMapAVL
+  Structures.OrderedTypeEx
+  FSets.FMapFacts
+  Compare_dec
+.
+
+Definition atom_lt (a1 a2 : atom) : Prop :=
+  match a1, a2 with
+  | A_lit c1, A_lit c2 => c1 < c2
+  | A_lit _, A_var _ => True
+  | A_var _, A_lit _ => False
+  | A_var v1, A_var v2 => v1 < v2
+  end.
+
+Module Atom_as_OT <: UsualOrderedType.
+
+  Definition t := atom.
+  Definition eq : atom -> atom -> Prop := @eq t.
+  Definition eq_refl := @eq_refl t.
+  Definition eq_sym := @eq_sym t.
+  Definition eq_trans := @eq_trans t.
+
+  Definition lt := atom_lt.
+
+  Lemma lt_trans : forall x y z, lt x y -> lt y z -> lt x z.
+  Proof.
+    intros x y z. destruct x, y, z; intros; simpl in *; auto.
+    - eapply Nat_as_OT.lt_trans; eauto.
+    - eapply Nat_as_OT.lt_trans; eauto.
+  Qed.
+
+  Lemma lt_not_eq : forall x y, lt x y -> ~eq x y.
+  Proof.
+    intros x y. destruct x, y; intros; unfold eq; simpl in *; auto.
+    - intros Hcontra. injection Hcontra; intros; lia.
+    - intros Hcontra. injection Hcontra; intros; lia.
+  Qed.
   
-  Record AList : Type :=
-    mkAList
-      { constants : list A;
-        varconsts : list A;
-        varvars : list (list A)
-      }.
-
-  (* How to represents variables in Gallina in here *)
-
+  Definition compare (x y : atom) : (@Compare atom lt eq x y).
+    destruct x, y.
+    - destruct (Nat_as_OT.compare c c0).
+      + assert (lt (A_lit c) (A_lit c0)).
+        {unfold lt, atom_lt. unfold Nat_as_OT.lt in *. lia. }
+        exact (LT H).
+      + assert (eq (A_lit c) (A_lit c0)).
+        {unfold eq. unfold Nat_as_OT.eq in *. subst; auto. }
+        exact (EQ H).
+      + assert (lt (A_lit c0) (A_lit c)).
+        {unfold lt, atom_lt. unfold Nat_as_OT.lt in *. lia. }
+        exact (GT H).
+    - assert (lt (A_lit c) (A_var x)) by (repeat red; auto).
+      exact (LT H).
+    - assert (lt (A_lit c) (A_var x)) by (repeat red; auto).
+      exact (GT H).
+    - destruct (Nat_as_OT.compare x x0).
+      + assert (lt (A_var x) (A_var x0)).
+        {unfold lt, atom_lt. unfold Nat_as_OT.lt in *. lia. }
+        exact (LT H).
+      + assert (eq (A_var x) (A_var x0)).
+        {unfold eq. unfold Nat_as_OT.eq in *. subst; auto. }
+        exact (EQ H).
+      + assert (lt (A_var x0) (A_var x)).
+        {unfold lt, atom_lt. unfold Nat_as_OT.lt in *. lia. }
+        exact (GT H).
+  Defined.
   
+  Definition eq_dec := eq_atom_dec.
+End Atom_as_OT.
+
+Definition atyp_lt (a1 a2 : atyp) : Prop :=
+  match a1 with
+  | AT_nil =>
+      match a2 with
+      | AT_nil => False
+      | _ => True
+      end
+  | AT_atom at1 =>
+      match a2 with
+      | AT_nil => False
+      | AT_atom at2 => Atom_as_OT.lt at1 at2
+      | _ => True
+      end
+  | AT_var v1 =>
+      match a2 with
+      | AT_var v2 => v1 < v2
+      | _ => False
+      end
+  end.
+
+Module Atyp_as_OT <: UsualOrderedType.
+
+  Definition t := atyp.
+  Definition eq := @eq t.
+  Definition eq_refl := @eq_refl t.
+  Definition eq_sym := @eq_sym t.
+  Definition eq_trans := @eq_trans t.
+
+  Definition lt := atyp_lt.
+
+  Lemma lt_trans : forall x y z, lt x y -> lt y z -> lt x z.
+  Proof.
+    intros x y z. destruct x, y, z; unfold lt, atom_lt; simpl in *; auto.
+    - apply Atom_as_OT.lt_trans.
+    - apply Nat_as_OT.lt_trans.
+  Qed.
+
+  Lemma lt_not_eq : forall x y, lt x y -> ~ eq x y.
+  Proof.
+    intros x y. destruct x, y; unfold lt, atom_lt, eq; intros; simpl in *; auto.
+    - intros Hcontra.  injection Hcontra; intros; subst.
+      apply Atom_as_OT.lt_not_eq in H.
+      unfold Atom_as_OT.eq in H.
+      specialize (H (Atom_as_OT.eq_refl a0)). inversion H.
+    - intros Hcontra. injection Hcontra; intros; subst.
+      apply Nat_as_OT.lt_not_eq in H.
+      unfold Nat_as_OT.eq in H.
+      specialize (H (Nat_as_OT.eq_refl x0)). inversion H.
+  Qed.
+
+  Definition compare x y : Compare lt eq x y.
+    destruct x, y.
+    - exact (EQ (eq_refl AT_nil)).
+    - assert (lt AT_nil (AT_atom a)) by (repeat red; auto).
+      exact (LT H).
+    - assert (lt AT_nil (AT_var x)) by (repeat red; auto).
+      exact (LT H).
+    - assert (lt AT_nil (AT_atom a)) by (repeat red; auto).
+      exact (GT H).
+    - destruct (Atom_as_OT.compare a a0).
+      + assert (lt (AT_atom a) (AT_atom a0)) by (repeat red in *; auto).
+        exact (LT H).
+      + assert (eq (AT_atom a) (AT_atom a0)). {repeat red in e; subst. repeat red.  auto. }
+        exact (EQ H).
+      + assert (lt (AT_atom a0) (AT_atom a)) by (repeat red in *; auto).
+        exact (GT H).
+    - assert (lt (AT_atom a) (AT_var x)) by (repeat red; auto).
+      exact (LT H).
+    - assert (lt AT_nil (AT_var x)) by (repeat red; auto).
+      exact (GT H).
+    - assert (lt (AT_atom a) (AT_var x)) by (repeat red; auto).
+      exact (GT H).
+    - destruct (Nat_as_OT.compare x x0).
+      + assert (lt (AT_var x) (AT_var x0)) by (repeat red in *; auto).
+        exact (LT H).
+      + assert (eq (AT_var x) (AT_var x0)). {repeat red in e; subst. repeat red.  auto. }
+        exact (EQ H).
+      + assert (lt (AT_var x0) (AT_var x)) by (repeat red in *; auto).
+        exact (GT H).
+  Defined.
+
+  Definition eq_dec := eq_atyp_dec.
+End Atyp_as_OT.
+
+Module NatMap := FMapAVL.Make(Nat_as_OT).
+(* Examples for using natmap *)
+Definition my_map := NatMap.add 1 42 (NatMap.empty _).
+Compute NatMap.find 1 my_map.
+Compute NatMap.find 2 my_map.
+Definition my_map_removed := NatMap.remove 1 my_map.
+Compute NatMap.find 1 my_map_removed.
+Module Facts := FMapFacts.WFacts_fun Nat_as_OT NatMap.
+Lemma find_add_eq : forall (k v : nat) m,
+  NatMap.find k (NatMap.add k v m) = Some v.
+Proof.
+  intros. apply Facts.find_mapsto_iff. apply NatMap.add_1. reflexivity.
+Qed.
+Section ReduceMap.
+  Notation lbag := (NatMap.t atyp).
+  Definition incr_count (a : atyp) (lbag : lbag) : lbag :=
+    match NatMap.find a lbag with
+    | None => NatMap.add a 1 lbag
+    | Some (c)
+  Definition list_to_lbag : list -> lbag :=
+    List.fold_right (fun a acc => NatMap.add)
+End ReduceMap.
+
+(* Section ReduceMap. *)
+(*   (* Convert to map *) *)
+(*   Context `{Countable A}. *)
+(*   Notation lbag := (gmultiset A). *)
+
+(*   (* Need to convert list to gmultiset  *)
+(*      Write a function that converts from gmultiset back to list, and argue that it's a permutation of the original list *)
+(*      Write a function that argues that if the original peqn is valid then converted and converted back is valid (should be a corollary from the above) *)
+(*      Write a reduce function *)
+(*      Argue that the original peqn is valid iff the reduced peqn is valid. *)
+(*    *) *)
+(*   Definition list_to_multiset (l : list atyp) : gmultiset A := *)
+(*     list_to_set_disj l. *)
   
-End AList.
- 
+(*   Definition pe_perm_to_multiset (l1 l2 : list atyp) : gmultiset A * gmultiset A := *)
+(*     (list_to_set_disj l1, list_to_set_disj l2). *)
+(*   (* Proof that if original peqn is valid then the converted peqn is valid *) *)
+(*   Lemma multiset_elements_perm : forall (l1 l2 : list atyp), l1 ≡[P] l2 -> elements (list_to_multiset l1) ≡[P] elements (list_to_multiset l2). *)
+(* End ReduceMap. *)
+
+Section Reification.
+  Equations reify (Σ : global_env_ext) (Γ : context) (P : term) : option form by (wf ())
+End Reification.
+  
